Arm/Memory/Separate.lean
@@ -230,12 +230,12 @@ theorem mem_legal'.omega_def (h : mem_legal' a n) : a.toNat + n ≤ 2^64 := h
 
 /-- The linear constraint is equivalent to `mem_legal'`. -/
 theorem mem_legal'.iff_omega (a : BitVec 64) (n : Nat) :
-    (a.toNat + n ≤ 2^64) ↔ mem_legal' a n := by
+    mem_legal' a n ↔ (a.toNat + n ≤ 2^64)  := by
   constructor
   · intros h
-    apply mem_legal'.of_omega h
-  · intros h
     apply h.omega_def
+  · intros h
+    apply mem_legal'.of_omega h
 
 instance : Decidable (mem_legal' a n) :=
   if h : a.toNat + n ≤ 2^64 then
@@ -341,14 +341,15 @@ theorem mem_separate'.of_omega
 
 /-- The linear constraint is equivalent to `mem_separate'`. -/
 theorem mem_separate'.iff_omega (a : BitVec 64) (an : Nat) (b : BitVec 64) (bn : Nat) :
+    mem_separate' a an b bn ↔
     (a.toNat + an ≤ 2^64 ∧
     b.toNat + bn ≤ 2^64 ∧
-    (a.toNat + an ≤ b.toNat ∨ a.toNat ≥ b.toNat + bn)) ↔ mem_separate' a an b bn := by
+    (a.toNat + an ≤ b.toNat ∨ a.toNat ≥ b.toNat + bn)) := by
   constructor
   · intros h
-    apply mem_separate'.of_omega h
-  · intros h
     apply h.omega_def
+  · intros h
+    apply mem_separate'.of_omega h
 
 instance : Decidable (mem_separate' a an b bn) :=
   if h : (a.toNat + an ≤ 2^64 ∧ b.toNat + bn ≤ 2^64 ∧ (a.toNat + an ≤ b.toNat ∨ a.toNat ≥ b.toNat + bn)) then
@@ -424,15 +425,16 @@ constructor
 
 /-- The linear constraint is equivalent to `mem_subset'`. -/
 theorem mem_subset'.iff_omega (a : BitVec 64) (an : Nat) (b : BitVec 64) (bn : Nat) :
+    mem_subset' a an b bn ↔
     (a.toNat + an ≤ 2^64 ∧
     b.toNat + bn ≤ 2^64 ∧
     b.toNat ≤ a.toNat ∧
-    a.toNat + an ≤ b.toNat + bn) ↔ mem_subset' a an b bn := by
+    a.toNat + an ≤ b.toNat + bn) := by
   constructor
   · intros h
-    apply mem_subset'.of_omega h
-  · intros h
     apply h.omega_def
+  · intros h
+    apply mem_subset'.of_omega h
 
 instance : Decidable (mem_subset' a an b bn) :=
   if h : (a.toNat + an ≤ 2^64 ∧ b.toNat + bn ≤ 2^64 ∧ b.toNat ≤ a.toNat ∧ a.toNat + an ≤ b.toNat + bn) then
